examples/low-level/stack.fst
@@ -1,35 +1,33 @@
 (*--build-config
-  other-files: list.fst
- --*)
+    options:--admit_fsi FStar.List --admit_fsi FStar.Set;
+    other-files:set.fsi ext.fst heap.fst st.fst all.fst list.fsi
+  --*)
+
+(** An implementation of a stack using the list module. *)
 
 module Stack
-(*#set-options "--initial_fuel 0 --max_fuel 0 --initial_ifuel 0 --max_ifuel 0"*)
-(*uncommenting the above fuel options seems to prevent Fstar from unfolding definitions in proofs*)
 
 open List
 
-type Stack (a:Type) = list a
+type stack (a:Type) = list a
 
-val push : #a:Type -> Stack a -> a -> Tot (Stack a)
+val push : #a:Type -> stack a -> a -> Tot (stack a)
 let push st e = e :: st
 
-
-val stail : #a:Type -> Stack a -> Tot (Stack a)
-let stail st =
+val tail : #a:Type -> stack a -> Tot (stack a)
+let tail st =
 match st with
 | [] -> []
 | h::tl -> tl
 
 let isNonEmpty = is_Cons
 
-val top : #a:Type -> l:(Stack a){ (isNonEmpty l)} -> Tot a
+val top : #a:Type -> l:stack a{isNonEmpty l} -> Tot a
 let top l =
 match l with
 | h::tl -> h
 
-val pop : #a:Type -> l:(Stack a){ (isNonEmpty l)} -> Tot (a * (Stack a))
+val pop : #a:Type -> l:stack a{isNonEmpty l} -> Tot (a * (stack a))
 let pop l =
 match l with
 | h::tl -> (h,tl)
-
-(*unlike Coq, match ... with.. does have an end*)
