examples/low-level/listset.fst
@@ -1,24 +1,26 @@
 (*--build-config
-    options:--admit_fsi FStar.Set;
-    other-files:ext.fst list.fst
+    options:--admit_fsi FStar.List --admit_fsi FStar.Set;
+    other-files:set.fsi ext.fst heap.fst st.fst all.fst list.fsi
   --*)
 
+(** Some extra helper functions for lists. *)
+
 module ListSet
+
 open FStar.List
 
-(*this is impossible to define unless equality on a is decidable.
-  the definition of memT does not seem to need a proof of decidability
-*)
-val lsubset :#a:Type -> list a -> list a -> Tot bool
+(** [lsubset la lb] is true if and only if all the elements from [la]
+    are also in [lb]. *)
+val lsubset: #a:Type -> list a -> list a -> Tot bool
 let rec lsubset la lb =
 match la with
 | [] -> true
 | h :: tl ->  ((mem h lb) && (lsubset tl lb))
 
-val notIn : #a:Type -> a-> list a  -> Tot bool
+val notIn : #a:Type -> a -> list a -> Tot bool
 let notIn id l = not (mem id l)
 
-val noRepeats :#a:Type -> list a  -> Tot bool
+val noRepeats : #a:Type -> list a -> Tot bool
 let rec noRepeats la =
 match la with
 | [] -> true
