examples/low-level/regions.fst
@@ -1,0 +1,486 @@
+(*--build-config
+    options:--admit_fsi FStar.Set;
+    other-files:ext.fst set.fsi heap.fst st.fst all.fst list.fst
+      stack.fst listset.fst ghost.fst located.fst lref.fst
+  --*)
+
+(* Note: we need the definitions of the functions from the [List]
+   module to reason about them, so not --admit_fsi for [FStar.List]. *)
+
+module Regions
+
+(** An axiomatization of regions in F* *)
+
+open FStar.Set
+open FStar.List
+open FStar.Ghost
+
+open ListSet
+open Located
+open Lref
+
+(** A region, taken individually, behaves just like a heap of its
+    own. Beware! This type is defined in [Lref] (it is *not* the
+    standard FStar heap type). *)
+type region = heap
+
+
+(* Recall that the [Located] module defines [rid], the type of
+   region-ids. In our axiomatization of regions, we carry around a
+   stack of regions where each region is tagged with an [rid]. This
+   axiomatization can be realized with two different models:
+   - one where [rid]s are globally unique throughout the entire
+     program execution, and
+   - one where [rid]s may be re-used.
+   The client code cannot assume one model or another (we're providing
+   the client with a weaker model than, say, one that guarantees that
+   [rid]s are never reused). This is similar to [ST] where the client
+   cannot assume either that memory locations will never be re-used. *)
+type regionStack = Stack.stack (rid * region)
+
+(* The naming convention is as follows: functions that operate on the
+   "stack" part of the memory end with [St], while functions that
+   operate on the [smem] type below end with [Mem]. *)
+val ridsSt : regionStack -> Tot (list rid)
+let ridsSt ms = mapT fst ms
+
+val wellFormed : regionStack -> Tot bool
+let wellFormed ms = noRepeats (ridsSt ms)
+
+(* A well-formed region stack is one where no [rid] appears twice. *)
+type wfRegionStack= x:regionStack{wellFormed x}
+
+
+(* The type of our memory: a garbage-collected heap along with a
+   custom-managed stack of regions. *)
+type smem = heap * wfRegionStack
+
+(* A series of helpers to work with the [smem] type. *)
+val hp : smem -> Tot heap
+let hp = fst
+
+val st : smem -> Tot wfRegionStack
+let st = snd
+
+val tail : smem -> Tot smem
+let tail (m : smem) =
+  hp m, Stack.tail (st m)
+
+val rids : smem -> Tot (list rid)
+let rids (m : smem) = ridsSt (st m)
+
+val topRegionAndId : s:smem{Stack.isNonEmpty (st s)} -> Tot (rid * region)
+let topRegionAndId ss = Stack.top (st ss)
+
+val topRegion : s:smem{Stack.isNonEmpty (st s)} -> Tot region
+let topRegion ss = snd (topRegionAndId ss)
+
+val topRegionId : s:smem{Stack.isNonEmpty (st s)} ->  Tot rid
+let topRegionId ss = fst (topRegionAndId ss)
+
+val refLoc : #a:Type -> lref a -> Tot regionLoc
+let refLoc r = regionOf r
+
+
+(* Find a region by [rid]. *)
+val regionById : rid  -> Stack.stack (rid * region) -> Tot (option region)
+let rec regionById id sp =
+  match sp with
+  | Nil -> None
+  | h::tl -> if id = fst h then Some (snd h) else regionById id tl
+
+(* Find a region by [regionLoc] (see [located.fst]). *)
+val regionByLoc : smem -> regionLoc -> Tot (option region)
+let regionByLoc m rl =
+  match rl with
+  | InHeap -> Some (hp m)
+  | InStack id -> regionById id (st m)
+
+(* A wrapper around [upd] (from [lref.fst]) that reverses the order of
+   the arguments, hence making it better suited to partial
+   application. *)
+val writeInRegion : #a:Type -> r:lref a -> v:a -> region -> Tot region
+let writeInRegion r v mb = upd mb r v
+
+(* Apply a function on a specific region in stack, leaving the rest
+   untouched. Typically used with a partial application of the
+   combinator above. *)
+val updateRegionById : (region -> Tot region)
+  -> rid
+  -> ms:regionStack
+  -> Tot (r:regionStack{ridsSt r = ridsSt ms})
+let rec updateRegionById f s ms=
+  match ms with
+  | [] -> []
+  | h::tl ->
+      if fst h = s then
+        (fst h, f (snd h))::tl
+       else
+         h::updateRegionById f s tl
+
+(* Write a new value in a reference that's in a given region id. *)
+val writeInMemStack : #a:Type -> lref a -> s:regionStack -> rid -> a -> Tot (r:regionStack{ridsSt r = ridsSt s})
+let rec writeInMemStack r ms s v = updateRegionById (writeInRegion r v) s ms
+
+
+// XXX JP: didn't proofread after that point. Lots of warnings.
+val changeStackBlockSameIDs :
+    f:(region -> Tot region) -> s:rid -> ms:(regionStack)
+  -> Lemma (ensures ((ridsSt ms) = (ridsSt (updateRegionById f s ms))))
+let rec changeStackBlockSameIDs f s ms =
+match ms with
+| Nil -> ()
+| h::tl ->   if (fst h = s) then () else (changeStackBlockSameIDs f s tl)
+
+val changeStackBlockWellFormed :
+ f:(region -> Tot region) -> s:rid -> ms:(regionStack)
+  -> Lemma
+      (requires (wellFormed ms))
+      (ensures (wellFormed (updateRegionById f s ms)))
+let changeStackBlockWellFormed  f s ms = (changeStackBlockSameIDs f s ms)
+
+val writeMemStackSameIDs : #a:Type -> r:(lref a) -> ms:(regionStack)
+  -> s:rid -> v:a
+  -> Lemma (ensures ((ridsSt ms) = (ridsSt (writeInMemStack r ms s v))))
+let writeMemStackSameIDs r ms s v = (changeStackBlockSameIDs (writeInRegion r v) s ms)
+
+val writeMemStackWellFormed : #a:Type -> r:(lref a)
+  -> ms:(regionStack)
+  -> s:rid -> v:a
+  -> Lemma
+      (requires (wellFormed (ms)))
+      (ensures (wellFormed (writeInMemStack r ms s v)))
+      [SMTPat (writeInMemStack r ms s v)]
+let writeMemStackWellFormed r ms s v = (changeStackBlockWellFormed (writeInRegion r v) s ms)
+
+(*val freeInMemStackSameIDs : #a:Type -> r:(lref a) -> ms:(regionStack)
+  -> s:rid
+  -> Lemma (ensures ((ridsSt ms) = (ridsSt (freeInMemStack r ms s))))
+let freeInMemStackSameIDs r ms s = (changeStackBlockSameIDs (freeRefInBlock r) s ms)
+
+val freeInMemStackWellFormed : #a:Type -> r:(lref a)
+  -> ms:(regionStack)
+  -> s:rid
+  -> Lemma
+      (requires (wellFormed (ms)))
+      (ensures (wellFormed (freeInMemStack r ms s)))
+      [SMTPat (freeInMemStack r ms s)]
+let freeInMemStackWellFormed r ms s = (changeStackBlockWellFormed (freeRefInBlock r) s ms)*)
+
+
+(*
+val writeMemStackSameStail : #a:Type -> r:(lref a) -> ms:(regionStack)
+  -> s:rid -> v:a
+  -> Lemma (ensures ((stail ms) = (stail (writeInMemStack r ms s v))))
+         (*  [SMTPat (writeMemStack r ms s v)] *)
+let rec writeMemStackSameStail r ms s v = ()
+*)
+
+
+val refExistsInStack : #a:Type -> (lref a)
+  -> id:rid -> (regionStack) -> Tot bool
+let rec refExistsInStack r id ms =
+match ms with
+| [] -> false
+| h::tl -> if (fst h=id) then (contains (snd h) r) else refExistsInStack r id tl
+
+
+val refExistsInStackId : #a:Type -> r:(lref a)
+  -> id:rid -> ms:(regionStack)
+  -> Lemma (requires (refExistsInStack r id ms))
+          (ensures (memT id (ridsSt ms)))
+let rec refExistsInStackId r id ms =
+match ms with
+| [] -> ()
+| h::tl -> if (fst h=id) then () else (refExistsInStackId r id tl)
+
+val memIdUniq:  h:(rid * region) -> tl:regionStack
+  -> Lemma (requires (wellFormed (h::tl)))
+        (ensures (notIn (fst h) (ridsSt tl)))
+let memIdUniq h tl = ()
+
+
+val refExistsInStackTail : #a:Type -> r:(lref a)
+  -> id:rid -> ms:wfRegionStack  -> Lemma (requires (refExistsInStack r id (Stack.tail ms)))
+          (ensures  (refExistsInStack r id ms))
+          [SMTPat (refExistsInStack r id (Stack.tail ms))]
+let refExistsInStackTail r id ms = (refExistsInStackId r id (Stack.tail ms))
+
+
+val liveRef : #a:Type -> (lref a) -> smem ->  Tot bool
+let liveRef (#a:Type) (r:lref a) (m:smem) =
+match (refLoc r) with
+| InHeap -> contains (hp m) r
+| InStack id -> refExistsInStack r id (st m)
+
+
+val writeMemStackExists : #a:Type -> #b:Type -> rw:(lref a) -> r: (lref b)
+  -> ms:(regionStack)
+  -> id:rid -> idw:rid -> v:a
+  -> Lemma
+      (requires (refExistsInStack r id ms))
+      (ensures (refExistsInStack r id (writeInMemStack rw ms idw v)))
+      [SMTPat (writeInMemStack rw ms id v)]
+let rec writeMemStackExists rw r ms id idw v =
+match ms with
+| Nil -> ()
+| h::tl ->   if (fst h = id) then () else ((writeMemStackExists rw r tl id idw v))
+
+
+val writeMemAux : #a:Type -> (lref a) -> m:smem -> a -> Tot (r:smem{rids r = rids m})
+let writeMemAux r m v =
+  match (refLoc r) with
+  | InHeap -> ((upd (hp m) r v), snd m)
+  | InStack id -> ( (hp m), (writeInMemStack r (st m) id v) )
+
+
+(*val freeMemAux : #a:Type -> (lref a) -> m:smem  -> Tot smem
+let freeMemAux r m =
+  match (refLoc r) with
+  | InHeap -> ((freeRefInBlock r (hp m)), snd m)
+  | InStack s -> ((hp m), ((freeInMemStack r (st m) s)))*)
+
+
+val writeMemAuxPreservesExists :  #a:Type -> #b:Type ->
+  rw:lref a -> r:lref b -> m:smem -> v:a ->
+Lemma (requires (liveRef r m))
+      (ensures (liveRef r (writeMemAux rw m v)))
+      [SMTPat (writeMemAux rw m v)]
+let writeMemAuxPreservesExists rw r m v =
+match (refLoc r) with
+| InHeap -> ()
+| InStack id ->
+    match (refLoc rw) with
+    | InHeap -> ()
+    | InStack idw ->  (writeMemStackExists rw r (st m) id idw v)
+
+
+val writeMemAuxPreserveridsSt :  #a:Type -> rw:lref a  -> m:smem -> v:a ->
+Lemma (requires (True)) (ensures (rids m = rids (writeMemAux rw m v)))
+ [SMTPat (writeMemAux rw m v)]
+
+let writeMemAuxPreserveridsSt rw m v =
+match (refLoc rw) with
+| InHeap -> ()
+| InStack id ->  (writeMemStackSameIDs rw (st m) id v)
+
+
+(*
+val writeMemAuxPreservesStail :  #a:Type -> r:(lref a) -> m:smem -> v:a ->
+Lemma (requires (is_InStack (refLoc r)))
+  (ensures tail m = tail (writeMemAux r m v))
+let rec writeMemAuxPreservesStail r m v =  ()
+*)
+
+val lookupRefStack : #a:Type -> r:(lref a) -> id:rid -> ms:(regionStack){refExistsInStack r id ms}  ->  Tot a
+let rec lookupRefStack r id ms =
+match ms with
+| h::tl ->
+    if (fst h = id) then  sel (snd h) r else (lookupRefStack r id tl)
+
+
+(* it is surprising that sel always returns something; It might be tricky to implement it.
+   What prevents me from creating a lref of an empty type? Perhaps it is impossible to create a member
+   of the type (lref False) . For example, the memory allocation operator, which creates a new (lref 'a)
+   requires an initial value of type 'a
+*)
+val lookupRef : #a:Type -> r:(lref a) -> m:smem{(liveRef r m) == true} ->  Tot a
+let lookupRef r m =
+match (refLoc r) with
+| InHeap -> (sel (hp m) r)
+| InStack id -> lookupRefStack r id (st m)
+
+
+type ifthenelseT (b:Type) (tc : Type) (fc: Type) =
+ (b ==>  tc) /\ ((~b) ==> fc )
+
+val readAfterWriteStack :
+  #a:Type  -> #b:Type -> rw:(lref a) -> r:(lref b) -> v:a -> id:rid -> idw:rid -> m:(regionStack) ->
+  Lemma (requires (refExistsInStack r id m))
+        (ensures ((refExistsInStack r id m)
+            /\ ifthenelseT (r==rw /\ id=idw)
+                (lookupRefStack r id (writeInMemStack rw m idw v) == v)
+                (lookupRefStack r id (writeInMemStack rw m idw v) = (lookupRefStack r id m))))
+let rec readAfterWriteStack rw r v id idw m =
+match m with
+| [] -> ()
+| h::tl ->
+  if (fst h = idw)
+    then ()
+    else (if (fst h=id)
+              then ()
+              else ((readAfterWriteStack rw r v id idw tl)))
+
+(*perhaps this specialization is not requires anymore*)
+val readAfterWriteStackSameType :
+  #a:Type -> rw:(lref a) -> r:(lref a) -> v:a -> id:rid -> idw:rid -> m:(regionStack) ->
+  Lemma (requires (refExistsInStack r id m))
+        (ensures ((refExistsInStack r id m)
+            /\ lookupRefStack r id (writeInMemStack rw m idw v) = (if (r=rw && id=idw) then v else (lookupRefStack r id m))))
+let readAfterWriteStackSameType rw r v id idw m = readAfterWriteStack rw r v id idw m
+
+val readAfterWrite : #a:Type -> #b:Type ->  rw:(lref a) -> r:(lref b) -> v:a -> m:smem ->
+  Lemma (requires (liveRef r m))
+        (ensures (liveRef r m)
+        /\ ifthenelseT (r==rw)
+            (lookupRef r (writeMemAux rw m v) == v)
+            (lookupRef r (writeMemAux rw m v) = (lookupRef r m)))
+let readAfterWrite rw r v m =
+match (refLoc r) with
+| InHeap -> ()
+| InStack id ->
+  match (refLoc rw) with
+  | InHeap -> ()
+  | InStack idw -> (readAfterWriteStack rw r v id idw (st m))
+
+(*Again, F*  does not seem to unfold ifthenelseT in the above. So, it seems
+necessary to provide the 2 specializations below as an SMTPat,
+instead of just the above lemma *)
+val readAfterWriteTrue : #a:Type -> #b:Type ->  rw:(lref a) -> r:(lref b) -> v:a -> m:smem ->
+  Lemma (requires (liveRef r m /\ r==rw))
+        (ensures (liveRef r m) /\
+            (lookupRef r (writeMemAux rw m v) == v))
+        [SMTPat (writeMemAux rw m v)]
+let readAfterWriteTrue rw r v m = readAfterWrite rw r v m
+
+
+val readAfterWriteFalse : #a:Type -> #b:Type ->  rw:(lref a) -> r:(lref b) -> v:a -> m:smem ->
+  Lemma (requires (liveRef r m /\ r=!=rw))
+        (ensures (liveRef r m) /\
+        (lookupRef r (writeMemAux rw m v) = (lookupRef r m)))
+        [SMTPat (writeMemAux rw m v)]
+let readAfterWriteFalse rw r v m = readAfterWrite rw r v m
+
+
+(*perhaps this specialization is not requires anymore*)
+val readAfterWriteSameType : #a:Type -> rw:(lref a) -> r:(lref a) -> v:a -> m:smem ->
+  Lemma (requires (liveRef r m))
+        (ensures (liveRef r m)
+            /\ lookupRef r (writeMemAux rw m v) = (if (r=rw) then v else (lookupRef r m)))
+let readAfterWriteSameType rw r v m = readAfterWrite rw r v m
+
+
+val liveRefTail : #a:Type -> r:(lref a) -> m:smem ->
+  Lemma (requires (liveRef r (tail m)))
+        (ensures (liveRef r (m)))
+        [SMTPat (liveRef r (tail m))]
+let liveRefTail r m =
+match (refLoc r) with
+| InHeap -> ()
+| InStack id -> (refExistsInStackTail r id (st m))
+
+val lookupRefStackTail
+  : #a:Type -> r:(lref a) -> id:rid -> m:wfRegionStack    ->  Lemma
+   (requires (refExistsInStack r id (Stack.tail m)))
+    (ensures ((refExistsInStack r id (Stack.tail m)) /\ lookupRefStack r id m
+        = lookupRefStack r id (Stack.tail m)))
+let lookupRefStackTail r id ms = (refExistsInStackId r id (Stack.tail ms))
+
+
+val readTailRef : #a:Type -> r:(lref a) -> m:smem ->
+  Lemma (requires (liveRef r (tail m)))
+        (ensures (liveRef r (tail m))
+            /\ lookupRef r m =  lookupRef r (tail m))
+            [SMTPat (liveRef r (tail m))]
+let readTailRef r m =
+match (refLoc r) with
+| InHeap -> ()
+| InStack id -> (lookupRefStackTail r id (st m))
+
+
+val writeStackTail
+  : #a:Type -> r:(lref a) -> id:rid -> v:a -> m:wfRegionStack    ->  Lemma
+      (requires (refExistsInStack r id (Stack.tail m)))
+      (ensures (Stack.tail (writeInMemStack r m id v)
+                    = writeInMemStack r (Stack.tail m) id v))
+let writeStackTail r id v ms = (refExistsInStackId r id (Stack.tail ms))
+
+val writeTailRef : #a:Type -> r:(lref a) -> m:smem -> v:a ->
+  Lemma (requires (liveRef r (tail m)))
+        (ensures (liveRef r (tail m))
+            /\ tail (writeMemAux r m v) =  writeMemAux r (tail m) v)
+            [SMTPat (liveRef r (tail m))]
+let writeTailRef r m v =
+match (refLoc r) with
+| InHeap -> ()
+| InStack id -> (writeStackTail r id v (st m))
+
+(* The location of a lref (say r) is refLoc r, and is independent of the
+   currrent state of the memory. So the absolute location of a reference is
+   by definition preserved by all memory operations.
+
+   However, in most correctness proofs, what matters is the relative position
+   w.r.t the top of the stack e.g.
+   whether the reference is in the tail of memory.
+   There are some memory operations that do not preserve relative position,
+   e.g. pushStackFrame.
+   However, most sane program blocks will preserve it. So far,
+   preserving stack ids is a definition of sanity
+   *)
+
+val liveRefSTailRids : #a:Type -> r:(lref a) -> id:rid  -> m0:wfRegionStack-> m1:wfRegionStack  -> Lemma
+   (requires (ridsSt m0 = ridsSt m1
+            /\ refExistsInStack r id (Stack.tail m0)
+            (*/\ refExistsInStack r id m0*)
+            /\ refExistsInStack r id m1))
+   (ensures refExistsInStack r id (Stack.tail m1))
+let liveRefSTailRids r id m0 m1 =
+(refExistsInStackId r id (Stack.tail m0))
+
+
+val liveRefTailRids : #a:Type -> r:(lref a) -> m0:smem -> m1:smem -> Lemma
+  (requires (rids m0 = rids m1 /\ liveRef r (tail m0) /\ liveRef r m1))
+  (ensures liveRef r (tail m1))
+  [SMTPat (rids m0 = rids m1)]
+let liveRefTailRids r m0 m1 =
+match (refLoc r) with
+| InHeap -> ()
+| InStack id -> (liveRefSTailRids r id (st m0) (st m1))
+
+
+
+(** modifiesOnly and lemmas about it*)
+
+(** cannot just uses ST.modifies. That was on heap; has to be lifted to smem.
+Also, why does it's definition have to be so procedural, unlike the more declarative one below?
+*)
+type canModify  (m0 : smem)  (m1: smem) (rs: modset ) =
+  forall (a:Type) (r: lref a).
+      liveRef r m0
+      ==> (~(Set.mem (Ref r) (reveal rs)))
+      ==> (liveRef r m1 /\ (lookupRef r m0 = lookupRef r m1))
+
+
+type  mreads (#a:Type) (r: lref a) (v:a) (m:smem) = liveRef r m /\ lookupRef r m = v
+
+(*lemmas needed for automatic inference*)
+val canModifyNone : m:smem -> Lemma (canModify m m (hide empty))
+let canModifyNone m = ()
+
+val canModifyWrite : #a:Type -> r:(lref a) -> v:a -> m:smem
+  -> Lemma (canModify m (writeMemAux r m v) (only  r))
+let canModifyWrite r v m = ()
+
+type mStackNonEmpty (m:smem) = b2t (Stack.isNonEmpty (st m))
+
+(*val canModifySalloc : #a:Type -> r:(lref a) -> v:a -> m:smem
+  -> Lemma (canModify m (writeMemAux r m v) (singleton (Ref r)))
+let canModifyWrite r v m = ()*)
+
+
+type allocateInBlock (#a:Type) (r: lref a) (h0 : region) (h1 : region) (init : a)   = not(contains h0 r) /\ contains h1 r /\  h1 == upd h0 r init
+
+val allocateInTopR: #a:Type -> r:lref a -> init:a -> m0:smem{Stack.isNonEmpty (st m0) /\
+                                                             not (contains (topRegion m0) r)}
+                    -> Tot smem
+let allocateInTopR r init m0 =
+    hp m0, (topRegionId m0, upd (topRegion m0) r init)::Stack.tail (st m0)
+
+
+(* liveness for arbitrary located data. It merely says that the stack id valid
+   This could be a much simpler definition for liveRef, if we agree to never (manually) free data.*)
+val liveLoc : #a:Type -> (located a) -> smem ->  Tot bool
+let liveLoc v m =
+  match (regionOf v) with
+  | InHeap -> true
+  | InStack id -> memT id  (rids m)
