examples/low-level/README.md
@@ -1,0 +1,13 @@
+A library for low-level, region-based allocation in F*.
+=======================================================
+
+Helpers:
+- stack.fst: an implementation of a stack using the list module
+- listset.fst: extra definitions related to lists
+
+Base files:
+- located.fst: base definitions for the `located` type
+- lref.fst: a bunch of lemmas ported from heap.fst so that they quantify over
+  our new located (ref a) type
+- regions.fst: an axiomatization of our stack of regions, along with a series of
+  lemmas
